# (c) Epimorphics Ltd, 2013

@prefix rdf:  <http://www.w3.org/1999/02/22-rdf-syntax-ns#> .
@prefix rdfs: <http://www.w3.org/2000/01/rdf-schema#> .
@prefix owl:  <http://www.w3.org/2002/07/owl#> .
@prefix xsd:  <http://www.w3.org/2001/XMLSchema#> .
@prefix dct:  <http://purl.org/dc/terms/> .
@prefix skos: <http://www.w3.org/2004/02/skos/core#> .
@prefix ui:   <http://purl.org/linked-data/registry-ui#> .

<http://purl.org/linked-data/registry-ui#>  a owl:Ontology;
    rdfs:label "Registry UI ontology"@en;
    rdfs:comment "Support for defining UI templates and form templates in RDF."@en;
    dct:contributor <http://www.amberdown.net/rdf/foaf.rdf#der> ;
    dct:created "2013-03-24"^^xsd:date;
    owl:versionInfo "0.1";
    .

# Form template

ui:FormTemplate a owl:Class;
    rdfs:label "Form Template"@en;
    rdfs:comment "Defines a kind of resource that can be instantiated via a form"@en;
    rdfs:subClassOf [owl:onProperty rdfs:label;       owl:minCardinality 1];
    rdfs:subClassOf [owl:onProperty ui:tooltip;       owl:minCardinality 0];
    rdfs:subClassOf [owl:onProperty ui:formFields;    owl:cardinality 1];
    rdfs:subClassOf [owl:onProperty ui:prototype;     owl:minCardinality 0];
    .

ui:formFields a owl:ObjectProperty;
    rdfs:label "form fields"@en;
    rdfs:comment "Indicates a list form fields which make up a template"@en;
    rdfs:domain ui:FormTemplate;
    rdfs:range  rdf:List;
    .

ui:prototype a owl:ObjectProperty;
    rdfs:label "prototype"@en;
    rdfs:comment "Indicates a resource whose property values should be copied to each instantiated resource generated by the form."@en;
    .

ui:tooltip a owl:DatatypeProperty;
    rdfs:label "tooltip"@en;
    rdfs:comment "Gives a tooltip which can be used to describe the a template or field";
    .

ui:FormField a owl:Class;
    rdfs:label "Form Field"@en;
    rdfs:comment "Defines a form field"@en;
    rdfs:subClassOf [owl:onProperty rdfs:label;       owl:minCardinality 1];
    rdfs:subClassOf [owl:onProperty ui:tooltip;       owl:minCardinality 0];
    rdfs:subClassOf [owl:onProperty ui:property;      owl:cardinality 1];
    rdfs:subClassOf [owl:onProperty ui:fieldType;     owl:cardinality 1];
    rdfs:subClassOf [owl:onProperty ui:required;      owl:minCardinality 0];
    rdfs:subClassOf [owl:onProperty ui:multivalued;   owl:minCardinality 0];
    # others in the future - required?  singleton?
    .

ui:property a owl:ObjectProperty;
    rdfs:label "property"@en;
    rdfs:comment "Indicates the property whose value will be given by this field"@en;
    rdfs:range rdf:Property;
    .

ui:multivalued a owl:DatatypeProperty;
    rdfs:label "required"@en;
    rdfs:comment "If true indicates that multiple values are allowed."@en;
    rdfs:range xsd:boolean;
    .

ui:required a owl:DatatypeProperty;
    rdfs:label "required"@en;
    rdfs:comment "If true indicates that the property values is required for a valid form"@en;
    rdfs:range xsd:boolean;
    .

ui:fieldType a owl:ObjectProperty;
    rdfs:label "field type"@en;
    rdfs:comment "Indicates the type of form field to be used, which in term defines the datatype of the generated value"@en;
    rdfs:range ui:FieldType;
    .

ui:FieldType a owl:Class;
    rdfs:label "Field Type"@en;
    rdfs:comment "Class of field type specifications"@en;
    .

ui:labelField a ui:FieldType; rdfs:label "label field"; rdfs:comment "Short text field" .
ui:textField a ui:FieldType; rdfs:label "text field"; rdfs:comment "Long text field" .
ui:anyURIField a ui:FieldType; rdfs:label "any uri field"; rdfs:comment "Manually entered URI for a resource" .

# Template entries

ui:Template a owl:Class;
    rdfs:label "Template"@en;
    rdfs:comment "Declaration of a type-specific rendering template"@en;
    .
    
ui:template a owl:DatatypeProperty;
    rdfs:label "template"@en;
    rdfs:comment "The relative file name of the template, normally ends with '.vm'"@en;
    rdfs:domain ui:Template;
    .
    
ui:type a owl:ObjectProperty;
    rdfs:label "type"@en;
    rdfs:comment "The resource type to which this template applies"@en;
    rdfs:domain ui:Template;
    rdfs:range  owl:Class;
    .
    
ui:templatePriority a owl:DatatypeProperty;
    rdfs:label "template priority"@en;
    rdfs:comment "The priority to give this template if multiple types match, high numbers indicate high priority"@en;
    rdfs:domain ui:Template;
    rdfs:range  xsd:int;
    .
    

